Append _def to definition theorems

regexScript.sml
@@ -10,7 +10,7 @@ val _ = Datatype `Reg = Eps | Sym 'a | Alt Reg Reg | Seq Reg Reg | Rep Reg`;
 
 (** Set-theoretic definition of what a regex matches. This is our ground truth. **)
 
-val language_of = Define `
+val language_of_def = Define `
   (language_of (Eps : 'a Reg) = {[]}) ∧
   (language_of (Sym x) = {[x]}) ∧
   (language_of (Alt a b) = language_of a ∪ language_of b) ∧
@@ -19,19 +19,19 @@ val language_of = Define `
 
 (** Naive, but executable, regex matcher. **)
 
-val split = Define `
+val split_def = Define `
   (split ([] : 'a list) = [([], [])]) ∧
   (split (c :: cs) = ([], c :: cs) :: MAP (CONS c ## I) (split cs)) `;
 
-val add_to_head = Define `
+val add_to_head_def = Define `
   (add_to_head (c : 'a) (x :: xs) = (c :: x) :: xs)`;
 
-val parts = Define `
+val parts_def = Define `
   (parts ([] : 'a list) = [[]]) ∧
   (parts [c] = [[[c]]]) ∧
   (parts (c :: cs) = MAP (CONS [c]) (parts cs) ++ MAP (add_to_head c) (parts cs)) `;
 
-val accept = Define `
+val accept_def = Define `
   (accept (Eps : 'a Reg) u = NULL u) ∧
   (accept (Sym c) u = (u = [c])) ∧
   (accept (Alt p q) u = accept p u ∨ accept q u) ∧
@@ -76,22 +76,22 @@ val _ = assert_false ``accept (Rep (Sym 1)) [1;2]``;
 
 val SPLIT_EMPTY1 = store_thm ("SPLIT_EMPTY1",
   ``∀ (a : 'a list). MEM ([], a) (split a)``,
-  Cases >> SIMP_TAC list_ss [split]);
+  Cases >> SIMP_TAC list_ss [split_def]);
 
 val SPLIT_SOUND = store_thm ("SPLIT_SOUND",
   ``∀ x y (w : 'a list). MEM (x, y) (split w) ⇒ (x ++ y = w)``,
   Induct_on `w` >| [
-    SIMP_TAC list_ss [split],
+    SIMP_TAC list_ss [split_def],
     REPEAT STRIP_TAC >>
-    FULL_SIMP_TAC list_ss [split, MEM_MAP, PAIR_MAP]
+    FULL_SIMP_TAC list_ss [split_def, MEM_MAP, PAIR_MAP]
   ]);
 
 val SPLIT_COMPLETE = store_thm ("SPLIT_COMPLETE",
   ``∀ a (b : 'a list). MEM (a, b) (split (a ++ b))``,
   Induct_on `a` >| [
-    SIMP_TAC list_ss [split, SPLIT_EMPTY1],
+    SIMP_TAC list_ss [split_def, SPLIT_EMPTY1],
 
-    SIMP_TAC list_ss [split] >>
+    SIMP_TAC list_ss [split_def] >>
     `∀ (b : 'a list) (f : 'a list # 'a list -> 'a list # 'a list).
       MEM (f (a,b)) (MAP f (split (a ++ b)))`
         suffices_by (
@@ -109,16 +109,16 @@ val PARTS_SOUND = store_thm ("PARTS_SOUND",
   ``∀ (li : 'a list) part. MEM part (parts li) ⇒ (FLAT part = li)``,
   Induct >| [
     REPEAT STRIP_TAC >>
-    FULL_SIMP_TAC list_ss [parts],
+    FULL_SIMP_TAC list_ss [parts_def],
 
     REPEAT STRIP_TAC >>
     Cases_on `li` >>
-    FULL_SIMP_TAC list_ss [parts, MEM_MAP] >>
+    FULL_SIMP_TAC list_ss [parts_def, MEM_MAP] >>
 
     `FLAT y = h'::t` by ASM_SIMP_TAC bool_ss[] >>
     Cases_on `y` >- FULL_SIMP_TAC list_ss [FLAT] >>
 
-    FULL_SIMP_TAC list_ss [add_to_head]
+    FULL_SIMP_TAC list_ss [add_to_head_def]
   ]);
 
 (* We'd want to say that parts is also complete in the sense that if we flatten
@@ -131,7 +131,7 @@ val PARTS_IN_FLAT = store_thm ("PARTS_IN_FLAT",
     ∀ (x : 'a list). MEM x part ⇒ MEM x li``,
   Induct >| [
     Q.EXISTS_TAC `[]` >>
-    ASM_SIMP_TAC list_ss [FLAT, parts],
+    ASM_SIMP_TAC list_ss [FLAT, parts_def],
 
     FULL_SIMP_TAC bool_ss [] >>
     Cases >| [
@@ -152,13 +152,13 @@ val PARTS_IN_FLAT = store_thm ("PARTS_IN_FLAT",
         Induct_on `t` >| [
           ASM_SIMP_TAC list_ss [] >>
           Cases_on `rest` >>
-          FULL_SIMP_TAC list_ss [parts, add_to_head] >>
+          FULL_SIMP_TAC list_ss [parts_def, add_to_head_def] >>
           Cases_on `t` >>
-          FULL_SIMP_TAC list_ss [parts, add_to_head, MEM_MAP] >>
-          METIS_TAC[parts, add_to_head],
+          FULL_SIMP_TAC list_ss [parts_def, add_to_head_def, MEM_MAP] >>
+          METIS_TAC[parts_def, add_to_head_def],
 
-          FULL_SIMP_TAC list_ss [parts, add_to_head] >>
-          METIS_TAC[parts, add_to_head, MEM_MAP]
+          FULL_SIMP_TAC list_ss [parts_def, add_to_head_def] >>
+          METIS_TAC[parts_def, add_to_head_def, MEM_MAP]
         ],
 
         FULL_SIMP_TAC list_ss []
@@ -170,13 +170,13 @@ val ACCEPT_SEQ_CONCAT = store_thm ("ACCEPT_SEQ_CONCAT",
   ``∀ p q u (v : 'a list).
     accept p u ∧ accept q v ⇒ accept (Seq p q) (u ++ v)``,
   REPEAT STRIP_TAC >>
-  SIMP_TAC list_ss [accept, EXISTS_MEM] >>
+  SIMP_TAC list_ss [accept_def, EXISTS_MEM] >>
   Q.EXISTS_TAC `(u, v)` >>
   ASM_SIMP_TAC std_ss [SPLIT_COMPLETE]);
 
 val ACCEPT_REP_NIL = store_thm ("ACCEPT_REP_NIL",
   ``∀ (p : 'a Reg). accept (Rep p) []``,
-  SIMP_TAC list_ss [accept, parts]);
+  SIMP_TAC list_ss [accept_def, parts_def]);
 
 (** Equivalence with language **)
 
@@ -185,7 +185,7 @@ val set_ss = std_ss ++ SET_SPEC_ss;
 val ACCEPT_IN_LANG = prove (
   ``∀ (r : 'a Reg) w. accept r w ⇒  w ∈ (language_of r)``,
   Induct >> REPEAT STRIP_TAC >>
-  FULL_SIMP_TAC set_ss [language_of, accept, IN_SING, IN_UNION, NULL] >| [
+  FULL_SIMP_TAC set_ss [language_of_def, accept_def, IN_SING, IN_UNION, NULL] >| [
     Cases_on `w` >> FULL_SIMP_TAC list_ss [],
 
     FULL_SIMP_TAC (std_ss ++ gen_beta_ss) [EXISTS_MEM] >>
@@ -201,8 +201,8 @@ val ACCEPT_IN_LANG = prove (
 val LANG_IN_ACCEPT = prove (
   ``∀ (r : 'a Reg) w. w ∈ (language_of r) ⇒ accept r w``,
   Induct >> REPEAT STRIP_TAC >>
-  FULL_SIMP_TAC set_ss [language_of, accept, IN_SING, IN_UNION, NULL] >| [
-    METIS_TAC [accept, ACCEPT_SEQ_CONCAT],
+  FULL_SIMP_TAC set_ss [language_of_def, accept_def, IN_SING, IN_UNION, NULL] >| [
+    METIS_TAC [accept_def, ACCEPT_SEQ_CONCAT],
 
     `∃ part. MEM part (parts (FLAT li)) ∧ ∀ x. (MEM x part ⇒ MEM x li)`
       by REWRITE_TAC [PARTS_IN_FLAT] >>
@@ -230,7 +230,7 @@ val _ = Datatype `
 
 (** Optimized-but-uncached regex matcher. **)
 
-val empty = Define `
+val empty_def = Define `
   (empty MEps = T) ∧
   (empty (MSym _ (_ : 'a)) = F) ∧
   (empty (MAlt p q) = empty p ∨ empty q) ∧
@@ -238,7 +238,7 @@ val empty = Define `
   (empty (MRep r) = T) ∧
   (empty (MInit _ r) = empty r)`;
 
-val final = Define `
+val final_def = Define `
   (final MEps = F) ∧
   (final (MSym b (_ : 'a)) = b) ∧
   (final (MAlt p q) = final p ∨ final q) ∧
@@ -246,7 +246,7 @@ val final = Define `
   (final (MRep r) = final r) ∧
   (final (MInit b r) = (b ∧ empty r) ∨ final r)`;
 
-val shift = Define `
+val shift_def = Define `
   (shift _ MEps _ = MEps) ∧
   (shift m (MSym _ x) c = MSym (m ∧ (x = c)) x) ∧
   (shift m (MAlt p q) c = MAlt (shift m p c) (shift m q c)) ∧
@@ -254,17 +254,17 @@ val shift = Define `
   (shift m (MRep r) c = MRep (shift (m ∨ final r) r c)) ∧
   (shift m (MInit b r) c = MInit F (shift (m ∨ b) r c))`;
 
-val acceptM = Define `
+val acceptM_def = Define `
   acceptM mr (s : 'a list) = final (FOLDL (shift F) (MInit T mr) s)`;
 
-val mark_reg = Define `
+val mark_reg_def = Define `
   (mark_reg Eps = MEps) ∧
   (mark_reg (Sym (c : 'a)) = MSym F c) ∧
   (mark_reg (Alt p q) = MAlt (mark_reg p) (mark_reg q)) ∧
   (mark_reg (Seq p q) = MSeq (mark_reg p) (mark_reg q)) ∧
   (mark_reg (Rep r) = MRep (mark_reg r)) `;
 
-val is_marked_reg = Define `
+val is_marked_reg_def = Define `
   (is_marked_reg Eps MEps = T) ∧
   (is_marked_reg (Sym (c : 'a)) (MSym _ mc) = (c = mc)) ∧
   (is_marked_reg (Alt p q) (MAlt mp mq) = is_marked_reg p mp ∧ is_marked_reg q mq) ∧
@@ -272,7 +272,7 @@ val is_marked_reg = Define `
   (is_marked_reg (Rep r) (MRep mr) = is_marked_reg r mr) ∧
   (is_marked_reg _ _ = F) `;
 
-val mark_le = Define `
+val mark_le_def = Define `
   (mark_le MEps MEps = T) ∧
   (mark_le (MSym ma (c : 'a)) (MSym mb d) = ((c = d) ∧ (ma ⇒ mb))) ∧
   (mark_le (MAlt p q) (MAlt mp mq) = mark_le p mp ∧ mark_le q mq) ∧
@@ -281,7 +281,7 @@ val mark_le = Define `
   (mark_le (MInit b1 r) (MInit b2 mr) = (b1 ⇒ b2) ∧ mark_le r mr) ∧
   (mark_le _ _ = F) `;
 
-val mark_union = Define `
+val mark_union_def = Define `
   (mark_union MEps MEps = MEps) ∧
   (mark_union (MSym ma (c : 'a)) (MSym mb _) = MSym (ma ∨ mb) c) ∧
   (mark_union (MAlt p q) (MAlt mp mq) = MAlt (mark_union p mp) (mark_union q mq)) ∧
@@ -291,7 +291,7 @@ val mark_union = Define `
 
 (** Some tests **)
 
-val _ = Define `accept2 r l = acceptM (mark_reg r) l`;
+val accept2_def = Define `accept2 r l = acceptM (mark_reg r) l`;
 
 val _ = assert_true ``empty (MAlt MEps (MEps : 'a MReg))``;
 val _ = assert_true ``empty (MAlt MEps (MSym T 2))``;
@@ -322,14 +322,14 @@ val _ = assert_false ``accept2 (Rep (Sym 1)) [1;2]``;
 
 val MARK_IS_MARKED = store_thm ("MARK_IS_MARKED",
   ``∀ (r : 'a Reg). is_marked_reg r (mark_reg r)``,
-  Induct >> ASM_REWRITE_TAC[mark_reg, is_marked_reg]);
+  Induct >> ASM_REWRITE_TAC[mark_reg_def, is_marked_reg_def]);
 
 val SHIFT_IS_MARKED = store_thm ("SHIFT_IS_MARKED",
   ``∀ (r : 'a Reg) mr m c.
     is_marked_reg r mr ⇒ is_marked_reg r (shift m mr c)``,
   Induct >> Cases_on `mr` >>
   REPEAT STRIP_TAC >>
-  FULL_SIMP_TAC bool_ss [shift, is_marked_reg]);
+  FULL_SIMP_TAC bool_ss [shift_def, is_marked_reg_def]);
 
 val FOLDL_SHIFT_IS_MARKED = prove (
   ``∀ (r : 'a Reg) mr m w.
@@ -343,7 +343,7 @@ val EMPTY_SOUND = store_thm ("EMPTY_SOUND",
   Induct >> Cases_on `mr` >>
   REPEAT STRIP_TAC >>
   FULL_SIMP_TAC (list_ss ++ SET_SPEC_ss ++ QI_ss)
-    [empty, is_marked_reg, language_of, IN_SING] >>
+    [empty_def, is_marked_reg_def, language_of_def, IN_SING] >>
   Q.EXISTS_TAC `[]` >>
   SIMP_TAC list_ss []);
 
@@ -351,35 +351,37 @@ val EMPTY_COMPLETE = store_thm ("EMPTY_COMPLETE",
   ``∀ r (mr : 'a MReg). [] ∈ language_of r ∧ is_marked_reg r mr ⇒ empty mr``,
   Induct >> Cases_on `mr` >>
   REPEAT STRIP_TAC >>
-  FULL_SIMP_TAC (list_ss ++ SET_SPEC_ss) [empty, is_marked_reg, language_of, IN_SING]);
+  FULL_SIMP_TAC (list_ss ++ SET_SPEC_ss) [empty_def, is_marked_reg_def, language_of_def, IN_SING]);
 
 val MARK_LE_REFL = store_thm ("MARK_LE_REFL",
   ``∀ (r : 'a MReg). mark_le r r``,
-  Induct >> ASM_REWRITE_TAC[mark_le]);
+  Induct >> ASM_REWRITE_TAC[mark_le_def]);
 
 val MARK_LE_TRANS = store_thm ("MARK_LE_TRANS",
   ``∀ r s (t : 'a MReg). mark_le r s ∧ mark_le s t ⇒ mark_le r t``,
   Induct >> Cases_on `s` >> Cases_on `t` >>
-  ASM_REWRITE_TAC [mark_le] >> METIS_TAC []);
+  ASM_REWRITE_TAC [mark_le_def] >> METIS_TAC []);
 
 val EMPTY_LE = store_thm ("EMPTY_LE",
   ``∀ r (s : 'a MReg). mark_le r s ⇒ (empty r = empty s)``,
   Induct >> Cases_on `s` >>
   REPEAT STRIP_TAC >>
-  FULL_SIMP_TAC bool_ss[mark_le, empty] >>
+  FULL_SIMP_TAC bool_ss[mark_le_def, empty_def] >>
   METIS_TAC[]);
 
 val FINAL_LE = store_thm ("FINAL_LE",
   ``∀ r (s : 'a MReg). mark_le r s ∧ final r ⇒ final s``,
   Induct >> Cases_on `s` >>
   REPEAT STRIP_TAC >>
-  FULL_SIMP_TAC bool_ss[mark_le, final] >>
+  FULL_SIMP_TAC bool_ss[mark_le_def, final_def] >>
   METIS_TAC [EMPTY_LE]);
 
 val SHIFT_LE = store_thm ("SHIFT_LE",
   ``∀ r s (c : 'a) b1 b2.
       (b1 ⇒ b2) ⇒ (mark_le r s) ⇒ mark_le (shift b1 r c) (shift b2 s c)``,
-  Induct >> Cases_on `s` >> REPEAT STRIP_TAC >> FULL_SIMP_TAC bool_ss[shift, mark_le] >>
+  Induct >> Cases_on `s` >>
+    REPEAT STRIP_TAC >>
+    FULL_SIMP_TAC bool_ss[shift_def, mark_le_def] >>
     `empty r = empty M` by (ASM_SIMP_TAC bool_ss [EMPTY_LE]) >>
     `(final r ⇒ final M)` by (METIS_TAC [FINAL_LE]) >>
     Cases_on `empty r` >> Cases_on `final r` >>
@@ -392,45 +394,45 @@ val MARK_REG_LE = store_thm ("MARK_REG_LE",
   ``∀ r (mr : 'a MReg). is_marked_reg r mr ⇒ mark_le (mark_reg r) mr``,
   Induct >> Cases_on `mr` >>
   REPEAT STRIP_TAC >>
-  FULL_SIMP_TAC bool_ss [is_marked_reg, mark_reg, mark_le]);
+  FULL_SIMP_TAC bool_ss [is_marked_reg_def, mark_reg_def, mark_le_def]);
 
 val IS_MARKED_REG_LE = store_thm ("IS_MARKED_REG_LE",
   ``∀ r mr (ms : 'a MReg). is_marked_reg r mr ∧ mark_le mr ms ⇒ is_marked_reg r ms``,
   Induct >> Cases_on `mr` >> Cases_on `ms` >>
-  ASM_SIMP_TAC bool_ss [is_marked_reg, mark_le] >>
+  ASM_SIMP_TAC bool_ss [is_marked_reg_def, mark_le_def] >>
   METIS_TAC []);
 
 val MARK_REG_NOT_FINAL = store_thm ("MARK_REG_NOT_FINAL",
   ``∀ (r : 'a Reg). ¬final (mark_reg r)``,
-  Induct >> FULL_SIMP_TAC bool_ss [mark_reg, final]);
+  Induct >> FULL_SIMP_TAC bool_ss [mark_reg_def, final_def]);
 
 val SHIFT_MARK_REG_F = store_thm ("SHIFT_MARK_REG_F",
   ``∀ (r : 'a Reg) c. shift F (mark_reg r) c = mark_reg r``,
-  Induct >> FULL_SIMP_TAC bool_ss [mark_reg, shift, MARK_REG_NOT_FINAL]);
+  Induct >> FULL_SIMP_TAC bool_ss [mark_reg_def, shift_def, MARK_REG_NOT_FINAL]);
 
 val FOLDL_MINIT_F = store_thm ("FOLDL_MINIT_F",
   ``∀ w (mr : 'a MReg).
     FOLDL (shift F) (MInit F mr) w = MInit F (FOLDL (shift F) mr w)``,
   INDUCT_THEN SNOC_INDUCT ASSUME_TAC >| [
     SIMP_TAC list_ss [],
-    ASM_SIMP_TAC list_ss [FOLDL_SNOC, shift]
+    ASM_SIMP_TAC list_ss [FOLDL_SNOC, shift_def]
   ]);
 
 val MARK_UNION_MARKED = store_thm ("MARK_UNION_MARKED",
   ``∀ (r : 'a Reg) ma mb.
     is_marked_reg r ma ∧ is_marked_reg r mb ⇒ is_marked_reg r (mark_union ma mb)``,
   Induct >> Cases_on `ma` >>
-  FULL_SIMP_TAC bool_ss [is_marked_reg] >>
+  FULL_SIMP_TAC bool_ss [is_marked_reg_def] >>
   Cases_on `mb` >>
-  FULL_SIMP_TAC bool_ss [is_marked_reg, mark_union]);
+  FULL_SIMP_TAC bool_ss [is_marked_reg_def, mark_union_def]);
 
 val IS_MARKED_EMPTY = store_thm ("IS_MARKED_EMPTY",
   ``∀ (r : 'a Reg) ma mb.
     is_marked_reg r ma ∧ is_marked_reg r mb ⇒ (empty ma = empty mb)``,
   Induct >> Cases_on `ma` >>
-  FULL_SIMP_TAC bool_ss [is_marked_reg] >>
+  FULL_SIMP_TAC bool_ss [is_marked_reg_def] >>
   Cases_on `mb` >>
-  FULL_SIMP_TAC bool_ss [is_marked_reg, empty] >>
+  FULL_SIMP_TAC bool_ss [is_marked_reg_def, empty_def] >>
   METIS_TAC[]);
 
 val MARK_UNION_FINAL = store_thm ("MARK_UNION_FINAL",
@@ -438,10 +440,10 @@ val MARK_UNION_FINAL = store_thm ("MARK_UNION_FINAL",
     is_marked_reg r ma ∧ is_marked_reg r mb ⇒
     (final (mark_union ma mb) = final ma ∨ final mb)``,
   Induct >> Cases_on `ma` >>
-  FULL_SIMP_TAC bool_ss [is_marked_reg] >>
+  FULL_SIMP_TAC bool_ss [is_marked_reg_def] >>
   Cases_on `mb` >>
-  FULL_SIMP_TAC bool_ss [is_marked_reg] >>
-  FULL_SIMP_TAC bool_ss [mark_union, final] >>
+  FULL_SIMP_TAC bool_ss [is_marked_reg_def] >>
+  FULL_SIMP_TAC bool_ss [mark_union_def, final_def] >>
   METIS_TAC[IS_MARKED_EMPTY, MARK_UNION_MARKED]);
 
 val MARK_UNION_EMPTY = store_thm ("MARK_UNION_EMPTY",
@@ -449,10 +451,10 @@ val MARK_UNION_EMPTY = store_thm ("MARK_UNION_EMPTY",
     is_marked_reg r ma ∧ is_marked_reg r mb ⇒
     (empty (mark_union ma mb) = empty ma)``,
   Induct >> Cases_on `ma` >>
-  FULL_SIMP_TAC bool_ss [is_marked_reg] >>
+  FULL_SIMP_TAC bool_ss [is_marked_reg_def] >>
   Cases_on `mb` >>
-  FULL_SIMP_TAC bool_ss [is_marked_reg] >>
-  FULL_SIMP_TAC bool_ss [mark_union, empty]);
+  FULL_SIMP_TAC bool_ss [is_marked_reg_def] >>
+  FULL_SIMP_TAC bool_ss [mark_union_def, empty_def]);
 
 val MARK_UNION_ID = store_thm ("MARK_UNION_ID",
   ``∀ (r : 'a Reg) ma.
@@ -464,20 +466,20 @@ val MARK_UNION_SHIFT = store_thm ("MARK_UNION_SHIFT",
     is_marked_reg r ma ∧ is_marked_reg r mb ⇒
     (mark_union (shift b1 ma c) (shift b2 mb c) = shift (b1 ∨ b2) (mark_union ma mb) c)``,
   Induct >> Cases_on `ma` >>
-  FULL_SIMP_TAC bool_ss [is_marked_reg] >>
+  FULL_SIMP_TAC bool_ss [is_marked_reg_def] >>
   Cases_on `mb` >>
-  FULL_SIMP_TAC bool_ss [is_marked_reg] >>
+  FULL_SIMP_TAC bool_ss [is_marked_reg_def] >>
   REPEAT STRIP_TAC >| [
-    FULL_SIMP_TAC bool_ss [mark_union, shift],
+    FULL_SIMP_TAC bool_ss [mark_union_def, shift_def],
 
-    FULL_SIMP_TAC bool_ss [mark_union, shift] >>
+    FULL_SIMP_TAC bool_ss [mark_union_def, shift_def] >>
     Cases_on `b1` >> Cases_on `b2` >> Cases_on `a' = c` >> SIMP_TAC bool_ss [],
 
-    FULL_SIMP_TAC bool_ss [mark_union, shift],
+    FULL_SIMP_TAC bool_ss [mark_union_def, shift_def],
 
     (* This is *terrible*. Is there no solver that handles booleans better?
      * Or at least is able to do boolean rewrites? *)
-    FULL_SIMP_TAC bool_ss [mark_union, shift] >>
+    FULL_SIMP_TAC bool_ss [mark_union_def, shift_def] >>
     RW_TAC bool_ss [] >>
     `empty (mark_union M M') = empty M` by METIS_TAC [MARK_UNION_EMPTY] >>
     `empty M' = empty M` by METIS_TAC [IS_MARKED_EMPTY] >>
@@ -486,7 +488,7 @@ val MARK_UNION_SHIFT = store_thm ("MARK_UNION_SHIFT",
     Cases_on `b1` >> Cases_on `b2` >> Cases_on `empty M` >>
     Cases_on `final M` >> Cases_on `final M'` >> ASM_SIMP_TAC bool_ss [],
 
-    FULL_SIMP_TAC bool_ss [mark_union, shift] >>
+    FULL_SIMP_TAC bool_ss [mark_union_def, shift_def] >>
     RW_TAC bool_ss [MARK_UNION_FINAL] >>
     cheat
   ]);
@@ -496,7 +498,7 @@ val MARK_UNION_SHIFT = store_thm ("MARK_UNION_SHIFT",
 val ACCEPTM_ALT = store_thm ("ACCEPTM_ALT",
   ``∀ p q (li : 'a list). (acceptM p li ∨ acceptM q li) ⇔ acceptM (MAlt p q) li``,
   NTAC 3 STRIP_TAC >>
-  FULL_SIMP_TAC bool_ss [acceptM] >>
+  FULL_SIMP_TAC bool_ss [acceptM_def] >>
   `∃ mp mq b.
     (FOLDL (shift F) (MInit T p) li = MInit b mp) ∧
     (FOLDL (shift F) (MInit T q) li = MInit b mq) ∧
@@ -506,17 +508,17 @@ val ACCEPTM_ALT = store_thm ("ACCEPTM_ALT",
       ASM_SIMP_TAC list_ss [] >>
       METIS_TAC [MARK_LE_REFL],
       STRIP_TAC >>
-      FULL_SIMP_TAC list_ss [shift, FOLDL_SNOC] >>
+      FULL_SIMP_TAC list_ss [shift_def, FOLDL_SNOC] >>
       RW_TAC (bool_ss ++ QI_ss) [SHIFT_LE]
     ]) >>
-  METIS_TAC [final, empty]);
+  METIS_TAC [final_def, empty_def]);
 
 val ACCEPTM_REP_APPEND = prove (
   ``∀ r x (y : 'a list).
     acceptM (MRep (mark_reg r)) x ∧ acceptM (mark_reg r) y ⇒
       acceptM (MRep (mark_reg r)) (x ++ y)``,
   REPEAT STRIP_TAC >>
-  FULL_SIMP_TAC list_ss [acceptM, FOLDL_APPEND] >>
+  FULL_SIMP_TAC list_ss [acceptM_def, FOLDL_APPEND] >>
 
   `∃ mr b. mark_le (mark_reg r) mr ∧
     (FOLDL (shift F) (MInit T (MRep (mark_reg r))) x = MInit b (MRep mr))` by (
@@ -526,7 +528,7 @@ val ACCEPTM_REP_APPEND = prove (
       METIS_TAC [MARK_LE_REFL],
 
       STRIP_TAC >>
-      FULL_SIMP_TAC list_ss [shift, FOLDL_SNOC] >>
+      FULL_SIMP_TAC list_ss [shift_def, FOLDL_SNOC] >>
       METIS_TAC [MARK_REG_LE, SHIFT_IS_MARKED, MARK_IS_MARKED, IS_MARKED_REG_LE]
     ]) >>
 
@@ -539,17 +541,17 @@ val ACCEPTM_REP_APPEND = prove (
     Q.ID_SPEC_TAC `y` >>
     INDUCT_THEN SNOC_INDUCT ASSUME_TAC >| [
       ASM_SIMP_TAC list_ss [] >>
-      METIS_TAC [final],
+      METIS_TAC [final_def],
 
       STRIP_TAC >>
-      FULL_SIMP_TAC list_ss [shift, FOLDL_SNOC] >>
+      FULL_SIMP_TAC list_ss [shift_def, FOLDL_SNOC] >>
       REPEAT (WEAKEN_TAC is_eq) >>
       RW_TAC (bool_ss ++ QI_ss) [] >>
       ASM_SIMP_TAC bool_ss [SHIFT_LE]
       (* It's odd that METIS isn't able to deal with this *)
     ]) >>
 
-  METIS_TAC [final, empty, FINAL_LE]);
+  METIS_TAC [final_def, empty_def, FINAL_LE]);
 
 val ACCEPTM_REP = prove (
   ``∀ r (li : 'a list list).
@@ -557,7 +559,7 @@ val ACCEPTM_REP = prove (
       acceptM (MRep (mark_reg r)) (FLAT li)``,
   STRIP_TAC >>
   INDUCT_THEN SNOC_INDUCT ASSUME_TAC >| [
-    FULL_SIMP_TAC list_ss [acceptM, empty, final],
+    FULL_SIMP_TAC list_ss [acceptM_def, empty_def, final_def],
     FULL_SIMP_TAC list_ss [FLAT_SNOC, ACCEPTM_REP_APPEND]
   ]);
 
@@ -566,7 +568,7 @@ val ACCEPTM_SEQ = prove (
     acceptM (mark_reg ra) x ∧ acceptM (mark_reg rb) y ⇒
       acceptM (MSeq (mark_reg ra) (mark_reg rb)) (x ++ y)``,
   REPEAT STRIP_TAC >>
-  FULL_SIMP_TAC list_ss [acceptM, FOLDL_APPEND] >>
+  FULL_SIMP_TAC list_ss [acceptM_def, FOLDL_APPEND] >>
 
   `∃ ma mb b. mark_le (mark_reg ra) ma ∧ mark_le (mark_reg rb) mb ∧
     (FOLDL (shift F) (MInit T (mark_reg ra)) x = MInit b ma) ∧
@@ -577,7 +579,7 @@ val ACCEPTM_SEQ = prove (
       METIS_TAC [MARK_LE_REFL],
 
       STRIP_TAC >>
-      FULL_SIMP_TAC list_ss [FOLDL_SNOC, shift] >>
+      FULL_SIMP_TAC list_ss [FOLDL_SNOC, shift_def] >>
       REPEAT (WEAKEN_TAC is_eq) >>
 
       Q.EXISTS_TAC `shift b ma x''` >>
@@ -596,24 +598,24 @@ val ACCEPTM_SEQ = prove (
     INDUCT_THEN SNOC_INDUCT ASSUME_TAC >| [
       ASM_SIMP_TAC list_ss [] >>
       RW_TAC (bool_ss ++ QI_ss) [] >>
-      FULL_SIMP_TAC bool_ss [final],
+      FULL_SIMP_TAC bool_ss [final_def],
 
       STRIP_TAC >>
-      FULL_SIMP_TAC list_ss [FOLDL_SNOC, shift] >>
+      FULL_SIMP_TAC list_ss [FOLDL_SNOC, shift_def] >>
       REPEAT (WEAKEN_TAC is_eq) >>
 
       RW_TAC (bool_ss ++ QI_ss) [SHIFT_LE]
     ]) >>
 
-  METIS_TAC [final, empty, FINAL_LE, EMPTY_LE]);
+  METIS_TAC [final_def, empty_def, FINAL_LE, EMPTY_LE]);
 
 val LANG_IN_ACCEPTM = prove (
   ``∀ (r : 'a Reg) w. w ∈ (language_of r) ⇒ acceptM (mark_reg r) w``,
   Induct >>
-  FULL_SIMP_TAC bool_ss [mark_reg, is_marked_reg, language_of] >>
+  FULL_SIMP_TAC bool_ss [mark_reg_def, is_marked_reg_def, language_of_def] >>
   REPEAT STRIP_TAC >| [
-    FULL_SIMP_TAC list_ss [IN_SING, acceptM, empty, final],
-    FULL_SIMP_TAC list_ss [IN_SING, acceptM, empty, final, shift],
+    FULL_SIMP_TAC list_ss [IN_SING, acceptM_def, empty_def, final_def],
+    FULL_SIMP_TAC list_ss [IN_SING, acceptM_def, empty_def, final_def, shift_def],
     METIS_TAC [IN_UNION, ACCEPTM_ALT],
     FULL_SIMP_TAC set_ss [ACCEPTM_SEQ],
     FULL_SIMP_TAC set_ss [ACCEPTM_REP]
@@ -627,10 +629,10 @@ val ACCEPTM_SEQ_SOUND = prove (
       acceptM (mark_reg r) y``,
   Induct >| [
     REPEAT STRIP_TAC >>
-    FULL_SIMP_TAC (list_ss ++ QI_ss) [acceptM, final, empty, MARK_REG_NOT_FINAL],
+    FULL_SIMP_TAC (list_ss ++ QI_ss) [acceptM_def, final_def, empty_def, MARK_REG_NOT_FINAL],
 
     REPEAT STRIP_TAC >>
-    FULL_SIMP_TAC list_ss [FOLDL, shift] >>
+    FULL_SIMP_TAC list_ss [FOLDL, shift_def] >>
 
     Q.ABBREV_TAC `acleft = b ∧ empty mr ∨ final mr` >>
     Q.ABBREV_TAC `right = (FOLDL (shift F) (shift T (mark_reg r) h) w)` >>
@@ -638,7 +640,7 @@ val ACCEPTM_SEQ_SOUND = prove (
     Cases_on `acleft ∧ final right` >| [
       Q.EXISTS_TAC `[]` >>
       Q.EXISTS_TAC `h :: w` >>
-      ASM_SIMP_TAC list_ss [final, acceptM, shift, FOLDL, FOLDL_MINIT_F],
+      ASM_SIMP_TAC list_ss [final_def, acceptM_def, shift_def, FOLDL, FOLDL_MINIT_F],
 
       `final (FOLDL (shift F) (MInit F (MSeq (shift b mr h) (mark_reg r))) w)` by (
         Cases_on `acleft` >| [
@@ -665,7 +667,7 @@ val ACCEPTM_SEQ_SOUND = prove (
                                SHIFT_IS_MARKED],
 
               STRIP_TAC >>
-              FULL_SIMP_TAC list_ss [FOLDL, FOLDL_SNOC, shift] >>
+              FULL_SIMP_TAC list_ss [FOLDL, FOLDL_SNOC, shift_def] >>
               Q.EXISTS_TAC `shift F ma x` >>
               Q.EXISTS_TAC `shift (final ma) mb' x` >>
               FULL_SIMP_TAC bool_ss [SHIFT_IS_MARKED] >>
@@ -696,19 +698,19 @@ val ACCEPTM_SEQ_SOUND = prove (
         by (ASM_SIMP_TAC bool_ss []) >>
       Q.EXISTS_TAC `h :: x` >>
       Q.EXISTS_TAC `y` >>
-      FULL_SIMP_TAC list_ss [shift]
+      FULL_SIMP_TAC list_ss [shift_def]
     ]
   ]);
 
 val ACCEPTM_IN_LANG = prove (
   ``∀ (r : 'a Reg) w. acceptM (mark_reg r) w ⇒ w ∈ (language_of r)``,
   Induct >>
-  FULL_SIMP_TAC bool_ss [language_of, IN_SING] >>
+  FULL_SIMP_TAC bool_ss [language_of_def, IN_SING] >>
   REPEAT STRIP_TAC >| [
     cheat,
     cheat,
 
-    FULL_SIMP_TAC set_ss [mark_reg, IN_UNION] >>
+    FULL_SIMP_TAC set_ss [mark_reg_def, IN_UNION] >>
     METIS_TAC [ACCEPTM_ALT],
 
     cheat,
